原文: https://zhuanlan.zhihu.com/p/582171443

$$
H = \sum_{\ev{ij}\in \alpha} = J_\alpha S_i^\alpha S_j^\alpha
$$

在马约拉纳表述下
$$
H = -\sum_{\ev{ij}\in \alpha} J_\alpha (\mi b_i^\alpha b_j^\alpha)
\mi c_i^\alpha c_j^\alpha
$$

令 $u_{ij} = \mi b_i^\alpha b_j^\alpha$

$$
H = -\sum_\alpha \sum_{\ev{ij}\in \alpha} J_\alpha u_{ij} \mi c_ic_j
$$

# 基态

令 $u_{ij} = 1$
$$
H = -\sum_\alpha \sum_{\ev{ij}\in \alpha} J_\alpha \mi c_ic_j
$$
做[[傅立叶变换|傅里叶变换]]
$$
c_i = \frac{1}{\sqrt{N}}\sum_k \me^{\mi \vb*{k}\vdot \vb*{r}_i} c_{k,A/B}
$$


