---
tags:
  - 量子力学
created: 2023-12-13 15:20:00
aliases:
  - adiabatic theorem
DOI: 
author: 
original title: 
year:
---
# 绝热定理证明

$$H \ket{\psi_n} = E_n \ket{\psi_n}$$
$$
H(t) \ket{\psi_n(t)} = E_n(t) \ket{\psi_n(t)}
$$
$$\psi_n(t) = \psi_n(0)\ \me^{-\mi E_n t/\hs}
\to \Psi(t) = \sum_n c_n(t) \psi_n(t)\ \me^{\mi \theta_n(t)}$$

$$
\Psi(t) = \sum_n c_n(t) \psi_n(t)\ \me^{-\frac{\mi}{\hs} \int_0^t E_n(t')\dd{t'}}
$$
其中
$$
\theta_n(t) \equiv -\frac{1}{\hs} \int_0^t E_n(t')\dd{t'}
$$

代入薛定谔方程
$$
-\mi\hs \pdv{t} \Psi(t) = H(t) \Psi(t)
$$
LHS:
$$
-\mi \hs \sum_n \qty[
\dot{c}_n \psi_n
+ c_n \dot{\psi}_n
+ \mi c_n \psi_n \dot{\theta}_n
]\me^{\mi \theta_n}
$$
根据 $\theta_n$ 的定义, 后两项消去.

RHS:
$$
\begin{align}
H(t) \Psi(t) &= H(t) \sum_n c_n \psi_n \me^{\mi \theta_n}\\
&= \sum_n c_n H(t) \psi_n \me^{\mi \theta_n}
\end{align}
$$

$$
\sum_n \me^{\mi \theta_n} \dot{c}_n \psi_n(t)
= -\sum_n c_n(t) \dot{\psi}_n \me^{\mi \theta_n}
$$

做内积

$$
\begin{align}
\sum_n \me^{\mi \theta_n} \dot{c}_n \ip{\psi_m}{\psi_n}
&= -\sum_n c_n \me^{\mi \theta_n} \ip*{\psi_m}{\dot{\psi}_n}\\
\dot{c}_m &= -\sum_n c_n(t) \ip*{\psi_m}{\dot{\psi}_n}\me^{\mi (\theta_n - \theta_m)}
\end{align}
$$

对 $H \psi_n = E_n \psi_n$ 求导
$$
\begin{align}
\dot{H} \psi_n + H \dot{\psi}_n
= \dot{E}_n \psi_n + E_n \dot{\psi}_n
\end{align}
$$
做内积
$$
\mel*{\psi_m}{\dot{H}}{\psi_n}
+E_m \ip*{\psi_m}{\dot{\psi}_n}
= \dot{E}_n \delta_{mn} + E_n \ip*{\psi_m}{\dot{\psi}_n}
$$
代入 $\dot{c}_m$ 表达式
$$
\dot{c}_m = -c_m \ip*{\psi_m}{\dot{\psi}_m}
- \sum_{n \neq m}
c_n \frac{\mel*{\psi_m}{\dot{H}}{\psi_n}}{E_n-E_m}\me^{\mi (\theta_n-\theta_m)}
$$
当 $H$ 变化率很小时, 省略求和
$$\dot{c}_m = -c_m \ip*{\psi_m}{\dot{\psi}_m}$$
通解为
$$
c_m(t) = c_m(0) \me^{\mi \gamma_m(t)}
$$
其中
$$
\gamma_m(t) = \mi \int_0^t
\ip{\psi_m(t')}{\pdv{t'} \psi_m(t')}\dd{t'}
$$




$$
\lim_{k \to \infty} \frac{\mel{v}{(H^k)^\dagger H^{k+1}}{v}}{\norm{H^k \ket{v}}^2} = E
$$